pcuic/theories/PCUICSN.v
@@ -8,7 +8,7 @@ From MetaCoq.PCUIC Require Import
 
 Require Import Equations.Prop.DepElim.
 
-(** We assume normalisation of the reduction.
+(** We assume normalization of the reduction.
     We state is as well-foundedness of the reduction.
 *)
 
@@ -40,15 +40,15 @@ Proof.
   all: trivial.
 Qed.
 
-Class NormalisationIn {cf : checker_flags} {no : normalizing_flags} (Σ : global_env_ext) :=
-  normalisation_in :
+Class NormalizationIn {cf : checker_flags} {no : normalizing_flags} (Σ : global_env_ext) :=
+  normalization_in :
     forall Γ t,
       welltyped Σ Γ t ->
       Acc (cored Σ Γ) t.
-Class Normalisation {cf : checker_flags} {no : normalizing_flags} :=
-  normalisation : forall Σ, wf_ext Σ -> NormalisationIn Σ.
-#[export] Hint Mode NormalisationIn - - + : typeclass_instances.
-#[export] Typeclasses Opaque Normalisation.
+Class Normalization {cf : checker_flags} {no : normalizing_flags} :=
+  normalization : forall Σ, wf_ext Σ -> NormalizationIn Σ.
+#[export] Hint Mode NormalizationIn - - + : typeclass_instances.
+#[export] Typeclasses Opaque Normalization.
 
 (** Since we are working with name annotations, reduction is sensitive to names.
     In this section we provide cored' which corresponds to reduction up to
@@ -59,7 +59,7 @@ Class Normalisation {cf : checker_flags} {no : normalizing_flags} :=
 Section Alpha.
 
   Context {cf : checker_flags} {no : normalizing_flags}.
-  Context (Σ : global_env_ext) {normalisation : NormalisationIn Σ}.
+  Context (Σ : global_env_ext) {normalization : NormalizationIn Σ}.
 
   Notation eqt u v := (∥ upto_names u v ∥).
 
@@ -159,13 +159,13 @@ Section Alpha.
     - destruct ee. constructor. symmetry; etransitivity; eassumption.
   Qed.
 
-  Lemma normalisation_upto :
+  Lemma normalization_upto :
     forall Γ u,
       welltyped Σ Γ u ->
       Acc (cored' Γ) u.
-  Proof using normalisation.
+  Proof using normalization.
     intros Γ u h.
-    apply normalisation in h.
+    apply normalization in h.
     eapply Acc_cored_cored'.
     - eassumption.
     - constructor; reflexivity.
