pcuic/theories/PCUICNormalization.v
@@ -21,12 +21,12 @@ From Equations Require Import Equations.
 
 From MetaCoq Require Import PCUICSN.
 
-Lemma wh_normalization {cf:checker_flags} {no:normalizing_flags} {Σ} {normalisation:NormalisationIn Σ} {t} : wf Σ -> axiom_free Σ ->
+Lemma wh_normalization {cf:checker_flags} {no:normalizing_flags} {Σ} {normalization:NormalizationIn Σ} {t} : wf Σ -> axiom_free Σ ->
 {A & Σ ;;; [] |- t : A}  -> { v & whnf RedFlags.default Σ [] v * red Σ [] t v}.
 Proof.
 intros Hwf Hax [A HA].
 assert (welltyped Σ [] t) as Hwt. { econstructor; eauto. }
-eapply PCUICSN.normalisation_in in Hwt as HSN; eauto. clear Hwt.
+eapply PCUICSN.normalization_in in Hwt as HSN; eauto. clear Hwt.
 induction HSN as [t H IH].
 edestruct progress_env_prop as [_ [_ [[t' Ht'] | Hval]]]; eauto.
 - eapply wcbv_red1_red1 in Ht' as Hred. 2:{ change 0 with (#|@nil context_decl|). eapply subject_closed. eauto. }
@@ -37,7 +37,7 @@ edestruct progress_env_prop as [_ [_ [[t' Ht'] | Hval]]]; eauto.
   eapply @subject_closed with (Γ := []); eauto.
 Defined.
 
-Lemma SN_to_WN {cf:checker_flags} {no:normalizing_flags} {Σ} {normalisation:NormalisationIn Σ} {A t} : wf Σ -> axiom_free Σ ->
+Lemma SN_to_WN {cf:checker_flags} {no:normalizing_flags} {Σ} {normalization:NormalizationIn Σ} {A t} : wf Σ -> axiom_free Σ ->
   Acc (cored Σ []) t -> Σ ;;; [] |- t : A -> { v & eval Σ t v}.
   intros Hwf Hax HSN HA.
   induction HSN as [t H IH].
@@ -50,12 +50,12 @@ Lemma SN_to_WN {cf:checker_flags} {no:normalizing_flags} {Σ} {normalisation:Nor
   - exists t. sq. eapply value_final; eauto.
 Qed.
 
-Lemma wcbv_normalization {cf:checker_flags} {no:normalizing_flags} {Σ} {normalisation:NormalisationIn Σ} {A t} : wf Σ -> axiom_free Σ ->
+Lemma wcbv_normalization {cf:checker_flags} {no:normalizing_flags} {Σ} {normalization:NormalizationIn Σ} {A t} : wf Σ -> axiom_free Σ ->
   Σ ;;; [] |- t : A -> { v & eval Σ t v}.
 Proof.
   intros Hwf Hax HA.
   assert (welltyped Σ [] t) as Hwt. { econstructor; eauto. }
-  eapply PCUICSN.normalisation_in in Hwt as HSN; eauto. clear Hwt.
+  eapply PCUICSN.normalization_in in Hwt as HSN; eauto. clear Hwt.
   eapply SN_to_WN; eauto.
 Qed.
 
@@ -96,14 +96,14 @@ Proof.
   - assert (x = y) as <- by eauto. eauto.
 Qed.
 
-Lemma ws_wcbv_standardization {cf:checker_flags} {no:normalizing_flags} {Σ} {normalisation:NormalisationIn Σ} {T} {t v : ws_term (fun _ => false)} : wf Σ -> axiom_free Σ ->
+Lemma ws_wcbv_standardization {cf:checker_flags} {no:normalizing_flags} {Σ} {normalization:NormalizationIn Σ} {T} {t v : ws_term (fun _ => false)} : wf Σ -> axiom_free Σ ->
   Σ ;;; [] |- t : T ->
   closed_red Σ [] t v ->
   ¬ { t' & Σ ;;; [] |- v ⇝ t'} ->
   {v' & eval Σ t v' * (Σ ;;; [] ⊢ v' ⇝ v)}.
 Proof.
   intros Hwf Hax Hty Hred Hirred.
-  destruct (@wcbv_normalization _ no Σ normalisation t) as (v' & Hv'); eauto.
+  destruct (@wcbv_normalization _ no Σ normalization T t) as (v' & Hv'); eauto.
   assert (Σ;;; [] |- t ⇝* v') as Hred' by now eapply wcbeval_red.
   eapply closed_red_confluence in Hred as Hred_. destruct Hred_ as (v'' & H1 & H2).
   2:{ econstructor; eauto. eapply subject_is_open_term. eauto. }
@@ -112,7 +112,7 @@ Proof.
   exists v'; split; eauto.
 Qed.
 
-Lemma ws_wcbv_standardization_fst {cf:checker_flags} {no:normalizing_flags} {Σ} {normalisation:NormalisationIn Σ} {i u args mind} {t v : ws_term (fun _ => false)} : wf Σ -> axiom_free Σ ->
+Lemma ws_wcbv_standardization_fst {cf:checker_flags} {no:normalizing_flags} {Σ} {normalization:NormalizationIn Σ} {i u args mind} {t v : ws_term (fun _ => false)} : wf Σ -> axiom_free Σ ->
   Σ ;;; [] |- t : mkApps (tInd i u) args ->
   lookup_env Σ (i.(inductive_mind)) = Some (InductiveDecl mind) ->
   @firstorder_ind Σ (firstorder_env Σ) i ->
@@ -133,7 +133,7 @@ Proof.
   Unshelve.
 Qed.
 
-Lemma wcbv_standardization {cf:checker_flags} {no:normalizing_flags} {Σ} {normalisation:NormalisationIn Σ} {T t v : term} : wf Σ -> axiom_free Σ ->
+Lemma wcbv_standardization {cf:checker_flags} {no:normalizing_flags} {Σ} {normalization:NormalizationIn Σ} {T t v : term} : wf Σ -> axiom_free Σ ->
   Σ ;;; [] |- t : T ->
   Σ ;;; [] |- t ⇝ v ->
   ¬ { t' & Σ ;;; [] |- v ⇝ t'} ->
@@ -152,7 +152,7 @@ Proof.
     eapply subject_reduction; eauto.
 Qed.
 
-Lemma wcbv_standardization_fst {cf:checker_flags} {no:normalizing_flags} {Σ} {normalisation:NormalisationIn Σ} {i u args mind} {t v : term} : wf Σ -> axiom_free Σ ->
+Lemma wcbv_standardization_fst {cf:checker_flags} {no:normalizing_flags} {Σ} {normalization:NormalizationIn Σ} {i u args mind} {t v : term} : wf Σ -> axiom_free Σ ->
   Σ ;;; [] |- t : mkApps (tInd i u) args ->
   lookup_env Σ (i.(inductive_mind)) = Some (InductiveDecl mind) ->
   @firstorder_ind Σ (firstorder_env Σ) i ->
