pcuic/theories/PCUICWeakeningConfigSN.v
@@ -3,14 +3,14 @@ From MetaCoq.Utils Require Import utils.
 From MetaCoq.PCUIC Require Import PCUICAst PCUICSN PCUICTyping PCUICSafeLemmata PCUICWeakeningConfigTyp.
 Import PCUICEnvironment.
 
-Lemma weakening_config_normalisation_in {cf1 cf2} {no1 no2}
+Lemma weakening_config_normalization_in {cf1 cf2} {no1 no2}
   Σ
   (Hcf : config.impl cf2 cf1)
-  : @PCUICSN.NormalisationIn cf1 no1 Σ -> @PCUICSN.NormalisationIn cf2 no2 Σ.
+  : @PCUICSN.NormalizationIn cf1 no1 Σ -> @PCUICSN.NormalizationIn cf2 no2 Σ.
 Proof.
-  cbv [PCUICSN.NormalisationIn].
-  intros normalisation_in Γ t1 [T Hwt]; specialize (normalisation_in Γ t1).
-  eapply Acc_incl; [ | eapply normalisation_in; econstructor; instantiate (1:=T); revert Hwt ].
+  cbv [PCUICSN.NormalizationIn].
+  intros normalization_in Γ t1 [T Hwt]; specialize (normalization_in Γ t1).
+  eapply Acc_incl; [ | eapply normalization_in; econstructor; instantiate (1:=T); revert Hwt ].
   { hnf; trivial. }
   eapply (@weakening_config cf2 cf1); assumption.
 Qed.
