pcuic/theories/PCUICWeakeningEnvSN.v
@@ -4,25 +4,25 @@ From MetaCoq.PCUIC Require Import PCUICAst PCUICSN PCUICTyping PCUICSafeLemmata 
 Import PCUICEnvironment.
 
 (* It would be nice to prove this, but I'm not sure how -Jason Gross *)
-Class NormalisationInAdjustUniversesIn {cf} {no} (Σ : global_env_ext) :=
-  normalisation_in_adjust_universes
+Class normalizationInAdjustUniversesIn {cf} {no} (Σ : global_env_ext) :=
+  normalization_in_adjust_universes
     : forall kn cb,
       lookup_env Σ.1 kn = Some (ConstantDecl cb) ->
       PCUICTyping.wf_ext Σ ->
       PCUICTyping.wf_ext (Σ.1, cst_universes cb) ->
-      @NormalisationIn cf no Σ -> @NormalisationIn cf no (Σ.1, cst_universes cb).
+      @NormalizationIn cf no Σ -> @NormalizationIn cf no (Σ.1, cst_universes cb).
 
-Lemma weakening_env_normalisation_in {cf} {no}
+Lemma weakening_env_normalization_in {cf} {no}
   Σ Σ' ϕ (Hext : extends Σ Σ')
   (HΣ : PCUICTyping.wf Σ)
   (HΣ' : PCUICTyping.wf Σ')
-  : @PCUICSN.NormalisationIn cf no (Σ', ϕ) -> @PCUICSN.NormalisationIn cf no (Σ, ϕ).
+  : @PCUICSN.NormalizationIn cf no (Σ', ϕ) -> @PCUICSN.NormalizationIn cf no (Σ, ϕ).
 Proof.
-  cbv [PCUICSN.NormalisationIn].
-  intros normalisation_in Γ t1 [T Hwt]; specialize (normalisation_in Γ t1); move: normalisation_in.
+  cbv [PCUICSN.NormalizationIn].
+  intros normalization_in Γ t1 [T Hwt]; specialize (normalization_in Γ t1); move: normalization_in.
   cbn in *.
-  move => normalisation_in.
-  eapply Acc_incl; [ | eapply normalisation_in; econstructor; instantiate (1:=T); revert Hwt ].
+  move => normalization_in.
+  eapply Acc_incl; [ | eapply normalization_in; econstructor; instantiate (1:=T); revert Hwt ].
   { repeat match goal with H : wf_ext _ |- _ => apply wf_ext_wf in H end.
     hnf; eapply weakening_env_cored; eassumption. }
   intro Hty.
