safechecker-plugin/theories/SafeTemplateChecker.v
@@ -22,7 +22,7 @@ Local Instance Monad_EnvCheck_wf_env_ext {cf:checker_flags} {guard : abstract_gu
 Program Definition infer_template_program {cf : checker_flags} {nor : normalizing_flags} {guard : abstract_guard_impl}
   (p : Ast.Env.program) φ
   (* this is the hypothesis we need, idk how to simplify it or appropriately generalize it, maybe use check_wf_env_ext_prop to simplify Σ0 ∼_ext X' into _ ∼ X so that we get an equality? *)
-  {normalisation_in
+  {normalization_in
     : forall (g : global_decl) (Hdecls' : nat) (X : X_env_type optimized_abstract_env_impl),
       (forall Σ0 : global_env,
           Σ0 ∼ X ->
@@ -34,11 +34,11 @@ Program Definition infer_template_program {cf : checker_flags} {nor : normalizin
             |}) ->
       forall X' : X_env_ext_type optimized_abstract_env_impl,
         check_wf_env_ext_prop optimized_abstract_env_impl X X' (universes_decl_of_decl g) ->
-        forall Σ0 : global_env_ext, wf_ext Σ0 -> Σ0 ∼_ext X' -> NormalisationIn Σ0}
-  {normalisation_in'
+        forall Σ0 : global_env_ext, wf_ext Σ0 -> Σ0 ∼_ext X' -> NormalizationIn Σ0}
+  {normalization_in'
     : forall x : X_env_ext_type optimized_abstract_env_impl,
       ((trans_program p).1, φ) ∼_ext x ->
-      forall Σ : global_env_ext, wf_ext Σ -> Σ ∼_ext x -> NormalisationIn Σ}
+      forall Σ : global_env_ext, wf_ext Σ -> Σ ∼_ext x -> NormalizationIn Σ}
   : EnvCheck_wf_env_ext (let p' := trans_program p in ∑ A, { X : wf_env_ext |
     ∥ (p'.1, φ) = X.(wf_env_ext_reference).(reference_impl_env_ext) × wf_ext (p'.1, φ) ×  (p'.1, φ) ;;; [] |- p'.2 : A ∥ }) :=
   pp <- typecheck_program (cf := cf) (nor:=nor) optimized_abstract_env_impl (trans_program p) φ ;;
@@ -50,7 +50,7 @@ Qed.
 Program Definition infer_and_print_template_program {cf : checker_flags} {nor : normalizing_flags} {guard : abstract_guard_impl}
   (p : Ast.Env.program) φ
 (* this is the hypothesis we need, idk how to simplify it or appropriately generalize it, maybe use check_wf_env_ext_prop to simplify Σ0 ∼_ext X' into _ ∼ X so that we get an equality? *)
-  {normalisation_in
+  {normalization_in
     : forall (g : global_decl) (Hdecls' : nat) (X : X_env_type optimized_abstract_env_impl),
       (forall Σ0 : global_env,
           Σ0 ∼ X ->
@@ -62,11 +62,11 @@ Program Definition infer_and_print_template_program {cf : checker_flags} {nor : 
             |}) ->
       forall X' : X_env_ext_type optimized_abstract_env_impl,
         check_wf_env_ext_prop optimized_abstract_env_impl X X' (universes_decl_of_decl g) ->
-        forall Σ0 : global_env_ext, wf_ext Σ0 -> Σ0 ∼_ext X' -> NormalisationIn Σ0}
-  {normalisation_in'
+        forall Σ0 : global_env_ext, wf_ext Σ0 -> Σ0 ∼_ext X' -> NormalizationIn Σ0}
+  {normalization_in'
     : forall x : X_env_ext_type optimized_abstract_env_impl,
       ((trans_program p).1, φ) ∼_ext x ->
-      forall Σ : global_env_ext, wf_ext Σ -> Σ ∼_ext x -> NormalisationIn Σ}  : string + string :=
+      forall Σ : global_env_ext, wf_ext Σ -> Σ ∼_ext x -> NormalizationIn Σ}  : string + string :=
   match infer_template_program (cf:=cf) p φ return string + string with
   | CorrectDecl t =>
     let Σ' := trans_global_env p.1 in
